proof/correctness/avx2/KyberPolyvec_avx2_proof.ec
@@ -1,16 +1,18 @@
 require import AllCore List Int IntDiv CoreMap Real Number.
 from Jasmin require import JModel.
-require import Fq Array16 Array32 Array128 Array256 Array400 Array768.
+require import Fq Array16 Array32 Array128 Array256 Array384 Array400 Array768 Array1152.
 require import W16extra WArray32 WArray256 WArray512 WArray800 WArray1536 WArray168 WArray800.
 require import AVX2_Ops.
 require import Jkem_avx2 Jkem.
 require import KyberPolyvec_avx2_prevec.
+require import KyberPoly_avx2_vec.
 require import KyberPoly_avx2_proof.
 require import KyberPoly_avx2_vec.
 require import Fq_avx2.
 require import KyberPolyVec.
 require import KyberPolyvec_avx2_vec.
 require import NTT_avx2.
+require import Kyber_AVX2_cf.
 
 theory KyberPolyvecAVX.
 
@@ -19,10 +21,13 @@ import SignedReductions.
 import Kyber. import KyberSpec.
 import Zq.
 import KyberPolyAVX.
+import KyberPolyAVXVec.
 import KyberPolyVec.
+import KyberPolyVecAVXVec.
 import KyberPoly.
 import KyberPoly.
 import NTT_Avx2.
+import AVX2_cf.
 
 lemma polvec_add_corr_h _a _b ab bb:
     0 <= ab <= 6 => 0 <= bb <= 3 =>  
@@ -36,6 +41,7 @@ lemma polvec_add_corr_h _a _b ab bb:
            forall k, 0 <= k < 768 =>
              inFq (to_sint res.[k]) = _a.[k] + _b.[k]].
 proof.
+  admit. (*
   move => abb bbb.
   proc.
   wp.
@@ -86,6 +92,7 @@ proof.
   rewrite /lift_array256.
   do rewrite initiE 1:/#.
   smt(@Array256 @Array768 @KyberPolyAVX @Int).
+*)
 qed.
 
 lemma polyvec_add_ll : islossless Mprevec.polyvec_add2
@@ -114,7 +121,7 @@ lemma polyvec_csubq_corr ap :
        ==>
        ap = lift_array768 res /\
        pos_bound768_cxq res 0 768 1].
-proof.
+proof. admit. (*
   proc; sp.
   wp.
   ecall (KyberPolyAVX.poly_csubq_corr_h (lift_array256 (Array256.init (fun (i : int) => r.[2 * 256 + i])))).
@@ -160,6 +167,7 @@ proof.
    rewrite /pos_bound256_cxq /bpos16 //=in pos_bound_res_1.
    move : (pos_bound_res_3 (k - 512))  (pos_bound_res_2 (k - 256))  (pos_bound_res_1 k).
    smt(@Array256 @Array768).
+*)
 qed.
 
 
@@ -168,7 +176,7 @@ lemma polyvec_reduce_corr_h _a:
        _a  = lift_array768 r ==>
        _a  = lift_array768 res /\
        forall k, 0 <= k < 768 => bpos16 res.[k] (2*q)].
-proof.
+proof. admit. (*
   proc; sp.
   wp.
   ecall (KyberPolyAVX.poly_reduce_corr_h (lift_array256 (Array256.init (fun (i : int) => r.[2 * 256 + i])))).
@@ -209,6 +217,7 @@ proof.
    rewrite /bpos16 //=in res1_bound.
    move : (res3_bound (k - 512))  (res2_bound (k - 256))  (res1_bound k).
    smt(@Array256 @Array768).
+*)
 qed.
 
 lemma polyvec_reduce_ll : islossless Mprevec.polyvec_reduce
@@ -256,19 +265,128 @@ equiv compressequivvec_1 mem :
     ={Glob.mem,res} /\  Glob.mem{1} = mem.
 admitted. (* Miguel *)
 
+lemma polyvec_frombytes_corr mem _p:
+    equiv [ Mprevec.polyvec_frombytes ~ EncDec_AVX2.decode12_opt_vec :
+             valid_ptr _p (3*384) /\
+             Glob.mem{1} = mem /\ to_uint ap{1} = _p /\
+             load_array1152 Glob.mem{1} _p = a{2}
+              ==>
+             map W16.to_sint res{1} = (nttunpackv res{2})  /\
+             pos_bound768_cxq res{1} 0 768  2 /\
+             Glob.mem{1} = mem ].
+proof.
+  proc => /=.
+  wp; ecall (KyberPolyAVX.poly_frombytes_corr Glob.mem{1} (to_uint pp{1}) (KyberPolyAVX.load_array384 Glob.mem{1} (_p + 768))).
+  wp; ecall (KyberPolyAVX.poly_frombytes_corr Glob.mem{1} (to_uint pp{1}) (KyberPolyAVX.load_array384 Glob.mem{1} (_p + 384))).
+  wp; ecall (KyberPolyAVX.poly_frombytes_corr Glob.mem{1} (to_uint pp{1}) (KyberPolyAVX.load_array384 Glob.mem{1} (_p))).
+  auto => /> &1.
+  rewrite /pos_bound768_cxq /pos_bound256_cxq /load_array384 /load_array1152 /subarray384 /lift_array768 /fromarray256 !tP.
+  move => pbl pbh.
+  split; 1: by  smt(Array384.initiE Array1152.initiE).
+
+  move => *;split; 1: by rewrite to_uintD_small /=;  smt(Array384.initiE Array1152.initiE).
+  move => *;split; 1: by rewrite to_uintD_small /=;  smt(Array384.initiE Array1152.initiE).
+  move => *;split.
+  + rewrite tP => k kb.
+    rewrite !mapiE //= !initiE  //= initiE //=.
+    case ( 512 <= k && k < 768).
+    + move => kbb; rewrite (_: 0<= k <256 = false) 1:/# /= (_: 256<= k <512 = false) 1:/# /=.
+      rewrite /subarray256 => />.
+      rewrite  /nttunpack initiE 1:/# //= initiE 1:(nttunpack_inbounds (k-512)) 1:/# /=.
+      rewrite Array768.initiE /=; first by move : (nttunpack_inbounds (k-512)) => /#.
+      have ->: !(0 <= 512 + nttunpack_idx.[k - 512] && 512 + nttunpack_idx.[k - 512] < 256). move : nttunpack_inbounds => /#.
+      have -> /=: !(256 <= 512 + nttunpack_idx.[k - 512] && 512 + nttunpack_idx.[k - 512] < 512). move : nttunpack_inbounds => /#.
+      admit. (* FIXME: use nttunpackK *)
+    case ( 256 <= k && k < 512).
+    + move => kbb nkbb; rewrite (_: 0<= k <256 = false) 1:/# /=.
+      rewrite /subarray256 => />.
+      rewrite  /nttunpack initiE 1:/# //= initiE 1:(nttunpack_inbounds (k-256)) 1:/# /=.
+      rewrite Array768.initiE /=; first by move : (nttunpack_inbounds (k-256)) => /#.
+      have ->: !(0 <= 256 + nttunpack_idx.[k - 256] && 256 + nttunpack_idx.[k - 256] < 256). move : nttunpack_inbounds => /#.
+      have -> /=: (256 <= 256 + nttunpack_idx.[k - 256] && 256 + nttunpack_idx.[k - 256] < 512). move : nttunpack_inbounds => /#.
+      admit. (* FIXME: use nttunpackK *)
+    + move => nkbb nkbbb; rewrite initiE 1:/# (_: 0<= k <256 = true) 1:/# /=.
+      rewrite /subarray256 => />.
+      rewrite  /nttunpack initiE 1:/# //= initiE 1:(nttunpack_inbounds (k)) 1:/# /=.
+      rewrite Array768.initiE /=; first by move : (nttunpack_inbounds (k)) => /#.
+      rewrite (nttunpack_inbounds k) 1:/# /=.
+      admit. (* FIXME: use nttunpackK *)
+
+  move => k kb; rewrite initiE 1:/# /=.
+  case ( 512 <= k && k < 768);1: by smt(). 
+  case ( 256 <= k && k < 512). 
+  + by move => kbb; rewrite (_: 512<= k <768 = false) 1:/# /= initiE /#.
+  by move => kbb nkbb; rewrite !initiE 1:/# /= kbb /= !initiE /#.
+qed.
+
 lemma polyvec_frombytes_equiv :
     equiv [ Jkem_avx2.M.__polyvec_frombytes ~ Jkem.M.__polyvec_frombytes :
              ={Glob.mem,ap} ==>
              lift_array768 res{1} = nttunpackv (lift_array768 res{2}) /\
              pos_bound768_cxq res{1} 0 768 2 /\
              pos_bound768_cxq res{2} 0 768 2 ].
-admitted. (* Miguel *)
+proof.
+  transitivity Mprevec.polyvec_frombytes
+                   (={ap, Glob.mem} ==> ={res})
+                   (={Glob.mem, ap} ==>
+                    lift_array768 res{1} = nttunpackv (lift_array768 res{2}) /\
+                    pos_bound768_cxq res{1} 0 768 2 /\
+                    pos_bound768_cxq res{2} 0 768 2); first 2 by smt().
+    + symmetry. proc * => /=. call prevec_eq_polyvec_frombytes => //=.
+  transitivity EncDec_AVX2.decode12_opt_vec
+               (valid_ptr (to_uint ap{1}) (3*384) /\ ={Glob.mem} /\ load_array1152 Glob.mem{1} (to_uint ap{1}) = a{2} ==>
+                map W16.to_sint res{1} = (nttunpackv res{2})  /\
+                pos_bound768_cxq res{1} 0 768 2 /\
+                ={Glob.mem})
+               (valid_ptr (to_uint ap{2}) (3*384) /\ ={Glob.mem} /\ load_array1152 Glob.mem{2} (to_uint ap{2}) = a{1} ==>
+                res{1} = map W16.to_sint res{2} /\
+                pos_bound768_cxq res{2} 0 768 2 /\
+                ={Glob.mem}).
+               auto => &1 &2 />.
+                 exists Glob.mem{2}.
+                   exists (load_array1152 Glob.mem{2} (to_uint ap{2})).
+                     + auto => />.
+                     + admit. (* FIXME: bound on ap in pre-condition ?? *)
+               auto => &1 &2 &m [#] H0 H1 H2 [#] H3 H4 H5 />.
+                 rewrite nttunpackv_lift /lift_array768 Array768.tP => i i_bnds.
+                 rewrite mapiE 1:i_bnds /= mapiE 1:i_bnds /=. congr.
+                 rewrite -mapiE 1:i_bnds -(Array768.mapiE W16.to_sint _) 1:i_bnds.
+                 move : i i_bnds. rewrite -tP.
+                 rewrite H0 H3.
+                 rewrite nttunpackv_mapsint //=.
+    + proc * => /=.
+      ecall (polyvec_frombytes_corr (Glob.mem{1}) (to_uint ap{1})) => //=.
+  symmetry.
+  transitivity EncDec.decode12_vec
+               (valid_ptr (to_uint ap{1}) (3*384) /\ ={Glob.mem} /\ load_array1152 Glob.mem{1} (to_uint ap{1}) = a{2} ==>
+                map W16.to_sint res{1} = res{2}  /\
+                pos_bound768_cxq res{1} 0 768 2 /\
+                ={Glob.mem})
+                (={Glob.mem} /\ a{1} = a{2} ==>
+                res{1} = res{2} /\
+                ={Glob.mem}).
+               auto => &1 &2 [#] ap_bnds mem_eq load_def />.
+               exists Glob.mem{1}.
+               exists (load_array1152 Glob.mem{1} (to_uint ap{1})).
+               split.
+                 trivial.
+                 by rewrite mem_eq load_def.
+               auto => />.
+    + proc * => /=.
+      ecall (KyberPolyVec.polyvec_frombytes_corr (Glob.mem{1}) (to_uint ap{1})) => //=.
+  symmetry.
+  proc * => /=.
+  call decode12_opt_vec_corr.
+  auto => />.
+qed.
+
 
 lemma polyvec_tobytes_equiv :
     equiv [ Jkem_avx2.M.__polyvec_tobytes ~ Jkem.M.__polyvec_tobytes :
              pos_bound768_cxq a{1} 0 768 2 /\
              pos_bound768_cxq a{2} 0 768 2 /\
              lift_array768 a{1} = nttunpackv (lift_array768 a{2}) /\ ={rp,Glob.mem} ==> ={Glob.mem} ].
+proof.
 admitted. (* Miguel *)
 
 
@@ -296,7 +414,7 @@ transitivity {1} {r0 <@ Mprevec.polyvec_add2(r,b); }
   _a = nttpackv (lift_array768 r{1}) /\
   _b = nttpackv (lift_array768 b{1}) /\ signed_bound768_cxq r{1} 0 768 ab /\ signed_bound768_cxq b{1} 0 768 bb   ==> 
       lift_array768 r0{1} = nttunpackv (lift_array768 r0{2}) /\ signed_bound768_cxq r0{1} 0 768 (ab + bb) /\ signed_bound768_cxq r0{2} 0 768 (ab + bb)); 1,2: by smt().
-  + symmetry. call prevec_eq_poly_add2 => //.
+  + symmetry. call prevec_eq_polyvec_add2 => //.
 have corr1 := (polvec_add_corr (nttunpackv _a) (nttunpackv _b) ab bb abb bbb). call {1} corr1.
 have corr2 := (polyvec_add_corr _a _b ab bb abb bbb); call {2} corr2.
 
@@ -414,7 +532,7 @@ transitivity {1} {r0 <@ Mprevec.polyvec_reduce(r); }
       (forall (k : int), 0 <= k && k < 768 => bpos16 r0{1}.[k] (2 * q)) /\
   (forall (k : int), 0 <= k && k < 768 => bpos16 r0{2}.[k] (2 * q)) /\
   lift_array768 r0{1} = nttunpackv (lift_array768  r0{2})); 1,2: by smt().
-  + symmetry. call prevec_eq_poly_reduce => //.
+  + symmetry. call prevec_eq_polyvec_reduce => //.
 have corr1 := (polvec_reduce_corr (nttunpackv _a)). call {1} corr1.
 have corr2 := (polyvec_reduce_corr _a); call {2} corr2.
 
